treiber -> treiber_stack. inf_chaselev -> inf_chaselev_deque.

theories/concurrent/inf_chaselev_deque.v
@@ -21,37 +21,37 @@ From caml5.std Require Import
 From caml5.concurrent Require Export
   base.
 
-Definition inf_chaselev_namespace :=
-  concurrent_namespace .@ "inf_chaselev".
+Definition inf_chaselev_deque_namespace :=
+  concurrent_namespace .@ "inf_chaselev_deque".
 
 Class InfChaselevGS Σ `{!heapGS Σ} (array : inf_array Σ) := {
-  inf_chaselev_GS_ctl_G : AuthExclG Σ (prodO ZO (nat -d> valO)) ;
-  inf_chaselev_GS_front_G : AuthNatMaxG Σ ;
-  inf_chaselev_GS_hist_G : mono_listG val Σ ;
-  inf_chaselev_GS_pub_G : AuthExclG Σ (listO valO) ;
-  inf_chaselev_GS_lock_G : ExclG Σ unitO ;
+  inf_chaselev_deque_GS_ctl_G : AuthExclG Σ (prodO ZO (nat -d> valO)) ;
+  inf_chaselev_deque_GS_front_G : AuthNatMaxG Σ ;
+  inf_chaselev_deque_GS_hist_G : mono_listG val Σ ;
+  inf_chaselev_deque_GS_pub_G : AuthExclG Σ (listO valO) ;
+  inf_chaselev_deque_GS_lock_G : ExclG Σ unitO ;
 }.
-#[local] Existing Instance inf_chaselev_GS_ctl_G.
-#[local] Existing Instance inf_chaselev_GS_front_G.
-#[local] Existing Instance inf_chaselev_GS_hist_G.
-#[local] Existing Instance inf_chaselev_GS_pub_G.
-#[local] Existing Instance inf_chaselev_GS_lock_G.
+#[local] Existing Instance inf_chaselev_deque_GS_ctl_G.
+#[local] Existing Instance inf_chaselev_deque_GS_front_G.
+#[local] Existing Instance inf_chaselev_deque_GS_hist_G.
+#[local] Existing Instance inf_chaselev_deque_GS_pub_G.
+#[local] Existing Instance inf_chaselev_deque_GS_lock_G.
 
-Definition inf_chaselev_Σ := #[
+Definition inf_chaselev_deque_Σ := #[
   auth_excl_Σ (prodO ZO (nat -d> valO)) ;
   auth_nat_max_Σ ;
   mono_listΣ val ;
   auth_excl_Σ (listO valO) ;
   excl_Σ unitO
 ].
-Lemma subG_inf_chaselev_Σ Σ `{!heapGS Σ} array :
-  subG inf_chaselev_Σ Σ →
+Lemma subG_inf_chaselev_deque_Σ Σ `{!heapGS Σ} array :
+  subG inf_chaselev_deque_Σ Σ →
   InfChaselevGS Σ array.
 Proof.
   solve_inG.
 Qed.
 
-Section inf_chaselev_GS.
+Section inf_chaselev_deque_GS.
   Context `{!heapGS Σ} {array} `{!InfChaselevGS Σ array}.
   Implicit Types front : nat.
   Implicit Types back : Z.
@@ -60,44 +60,44 @@ Section inf_chaselev_GS.
   Implicit Types hist pub : list val.
   Implicit Types priv : nat → val.
 
-  Notation inf_chaselev_offset_front := 0%Z.
-  Notation inf_chaselev_offset_back := 1%Z.
-  Notation inf_chaselev_offset_array := 2%Z.
+  Notation inf_chaselev_deque_offset_front := 0%Z.
+  Notation inf_chaselev_deque_offset_back := 1%Z.
+  Notation inf_chaselev_deque_offset_array := 2%Z.
 
-  Notation "t '.(front)'" := (t +ₗ inf_chaselev_offset_front)%stdpp
+  Notation "t '.(front)'" := (t +ₗ inf_chaselev_deque_offset_front)%stdpp
   ( at level 5
   ) : stdpp_scope.
-  Notation "t '.(back)'" := (t +ₗ inf_chaselev_offset_back)%stdpp
+  Notation "t '.(back)'" := (t +ₗ inf_chaselev_deque_offset_back)%stdpp
   ( at level 5
   ) : stdpp_scope.
-  Notation "t '.(array)'" := (t +ₗ inf_chaselev_offset_array)%stdpp
+  Notation "t '.(array)'" := (t +ₗ inf_chaselev_deque_offset_array)%stdpp
   ( at level 5
   ) : stdpp_scope.
-  Notation "t '.(front)'" := (t +ₗ #inf_chaselev_offset_front)%E
+  Notation "t '.(front)'" := (t +ₗ #inf_chaselev_deque_offset_front)%E
   ( at level 5
   ) : expr_scope.
-  Notation "t '.(back)'" := (t +ₗ #inf_chaselev_offset_back)%E
+  Notation "t '.(back)'" := (t +ₗ #inf_chaselev_deque_offset_back)%E
   ( at level 5
   ) : expr_scope.
-  Notation "t '.(array)'" := (t +ₗ #inf_chaselev_offset_array)%E
+  Notation "t '.(array)'" := (t +ₗ #inf_chaselev_deque_offset_array)%E
   ( at level 5
   ) : expr_scope.
 
-  Definition inf_chaselev_make : val :=
+  Definition inf_chaselev_deque_make : val :=
     λ: <>,
       let: "t" := AllocN #3 #0 in
       "t".(array) <- array.(inf_array_make) #() ;;
       "t".
 
-  Definition inf_chaselev_push : val :=
+  Definition inf_chaselev_deque_push : val :=
     λ: "t" "v",
       let: "back" := !"t".(back) in
       let: "arr" := !"t".(array) in
       array.(inf_array_set) "arr" "back" "v" ;;
       "t".(back) <- "back" + #1.
 
-  Definition inf_chaselev_steal : val :=
-    rec: "inf_chaselev_steal" "t" :=
+  Definition inf_chaselev_deque_steal : val :=
+    rec: "inf_chaselev_deque_steal" "t" :=
       let: "front" := !"t".(front) in
       let: "back" := !"t".(back) in
       let: "arr" := !"t".(array) in
@@ -106,13 +106,13 @@ Section inf_chaselev_GS.
         if: CAS "t".(front) "front" ("front" + #1) then (
           SOME "v"
         ) else (
-          "inf_chaselev_steal" "t"
+          "inf_chaselev_deque_steal" "t"
         )
       ) else (
         NONE
       ).
 
-  Definition inf_chaselev_pop : val :=
+  Definition inf_chaselev_deque_pop : val :=
     λ: "t",
       let: "back" := !"t".(back) - #1 in
       let: "arr" := !"t".(array) in
@@ -136,255 +136,255 @@ Section inf_chaselev_GS.
         )
       ).
 
-  Notation inf_chaselev_meta_ctl := (nroot .@ "ctl").
-  Notation inf_chaselev_meta_front := (nroot .@ "front").
-  Notation inf_chaselev_meta_hist := (nroot .@ "hist").
-  Notation inf_chaselev_meta_pub := (nroot .@ "pub").
-  Notation inf_chaselev_meta_lock := (nroot .@ "lock").
+  Notation inf_chaselev_deque_meta_ctl := (nroot .@ "ctl").
+  Notation inf_chaselev_deque_meta_front := (nroot .@ "front").
+  Notation inf_chaselev_deque_meta_hist := (nroot .@ "hist").
+  Notation inf_chaselev_deque_meta_pub := (nroot .@ "pub").
+  Notation inf_chaselev_deque_meta_lock := (nroot .@ "lock").
 
-  #[local] Definition inf_chaselev_ctl₁ γ_ctl back priv :=
-    @auth_excl_auth _ _ inf_chaselev_GS_ctl_G γ_ctl (DfracOwn 1) (back, priv).
-  #[local] Definition inf_chaselev_ctl₂ γ_ctl back priv :=
-    @auth_excl_frag _ _ inf_chaselev_GS_ctl_G γ_ctl (back, priv).
+  #[local] Definition inf_chaselev_deque_ctl₁ γ_ctl back priv :=
+    @auth_excl_auth _ _ inf_chaselev_deque_GS_ctl_G γ_ctl (DfracOwn 1) (back, priv).
+  #[local] Definition inf_chaselev_deque_ctl₂ γ_ctl back priv :=
+    @auth_excl_frag _ _ inf_chaselev_deque_GS_ctl_G γ_ctl (back, priv).
 
-  #[local] Definition inf_chaselev_front_auth γ_front front :=
+  #[local] Definition inf_chaselev_deque_front_auth γ_front front :=
     auth_nat_max_auth γ_front (DfracOwn 1) front.
-  #[local] Definition inf_chaselev_front_frag γ_front front :=
+  #[local] Definition inf_chaselev_deque_front_frag γ_front front :=
     auth_nat_max_frag γ_front front.
 
-  #[local] Definition inf_chaselev_hist_auth γ_hist hist pub :=
+  #[local] Definition inf_chaselev_deque_hist_auth γ_hist hist pub :=
     mono_list_auth_own γ_hist 1
       match pub with
       | [] => hist
       | v :: _ => hist ++ [v]
       end.
-  #[local] Definition inf_chaselev_hist_frag γ_hist i v :=
+  #[local] Definition inf_chaselev_deque_hist_frag γ_hist i v :=
     mono_list_idx_own γ_hist i v.
 
-  #[local] Definition inf_chaselev_pub₁ γ_pub pub :=
-    @auth_excl_frag _ _ inf_chaselev_GS_pub_G γ_pub pub.
-  #[local] Definition inf_chaselev_pub₂ γ_pub pub :=
-    @auth_excl_auth _ _ inf_chaselev_GS_pub_G γ_pub (DfracOwn 1) pub.
+  #[local] Definition inf_chaselev_deque_pub₁ γ_pub pub :=
+    @auth_excl_frag _ _ inf_chaselev_deque_GS_pub_G γ_pub pub.
+  #[local] Definition inf_chaselev_deque_pub₂ γ_pub pub :=
+    @auth_excl_auth _ _ inf_chaselev_deque_GS_pub_G γ_pub (DfracOwn 1) pub.
 
-  #[local] Definition inf_chaselev_lock γ_lock :=
+  #[local] Definition inf_chaselev_deque_lock γ_lock :=
     excl γ_lock ().
 
-  #[local] Definition inf_chaselev_state₁ front back pub : iProp Σ :=
+  #[local] Definition inf_chaselev_deque_state₁ front back pub : iProp Σ :=
     ⌜(front ≤ back)%Z ∧ length pub = Z.to_nat (back - front)⌝.
-  #[local] Definition inf_chaselev_state₂₁ front back pub : iProp Σ :=
+  #[local] Definition inf_chaselev_deque_state₂₁ front back pub : iProp Σ :=
     ⌜back = front ∧ length pub = 1⌝.
-  #[local] Definition inf_chaselev_state₂₂ front back pub : iProp Σ :=
+  #[local] Definition inf_chaselev_deque_state₂₂ front back pub : iProp Σ :=
     ⌜Z.of_nat front = (back + 1)%Z ∧ pub = []⌝.
-  #[local] Definition inf_chaselev_state₂ γ_lock front back pub : iProp Σ :=
-    inf_chaselev_lock γ_lock ∗
-    (inf_chaselev_state₂₁ front back pub ∨ inf_chaselev_state₂₂ front back pub).
-  #[local] Definition inf_chaselev_state γ_lock front back pub : iProp Σ :=
-    inf_chaselev_state₁ front back pub ∨
-    inf_chaselev_state₂ γ_lock front back pub.
+  #[local] Definition inf_chaselev_deque_state₂ γ_lock front back pub : iProp Σ :=
+    inf_chaselev_deque_lock γ_lock ∗
+    (inf_chaselev_deque_state₂₁ front back pub ∨ inf_chaselev_deque_state₂₂ front back pub).
+  #[local] Definition inf_chaselev_deque_state γ_lock front back pub : iProp Σ :=
+    inf_chaselev_deque_state₁ front back pub ∨
+    inf_chaselev_deque_state₂ γ_lock front back pub.
 
-  #[local] Definition inf_chaselev_array_model arr hist pub priv :=
+  #[local] Definition inf_chaselev_deque_array_model arr hist pub priv :=
     array.(inf_array_model) arr (
       λ i,
         let vs := hist ++ pub in
         if decide (i < length vs) then vs !!! i else priv (i - length vs)
     ).
 
-  #[local] Definition inf_chaselev_inv_inner l γ_ctl γ_front γ_hist γ_pub γ_lock arr : iProp Σ :=
+  #[local] Definition inf_chaselev_deque_inv_inner l γ_ctl γ_front γ_hist γ_pub γ_lock arr : iProp Σ :=
     ∃ front back hist pub priv,
     (* physical fields *)
     l.(front) ↦ #front ∗ l.(back) ↦ #back ∗
     (* control token *)
-    inf_chaselev_ctl₁ γ_ctl back priv ∗
+    inf_chaselev_deque_ctl₁ γ_ctl back priv ∗
     (* front authority *)
-    inf_chaselev_front_auth γ_front front ∗
+    inf_chaselev_deque_front_auth γ_front front ∗
     (* array contents *)
-    inf_chaselev_array_model arr hist pub priv ∗
+    inf_chaselev_deque_array_model arr hist pub priv ∗
     (* history values *)
     ⌜length hist = front⌝ ∗
-    inf_chaselev_hist_auth γ_hist hist pub ∗
+    inf_chaselev_deque_hist_auth γ_hist hist pub ∗
     (* public values *)
-    inf_chaselev_pub₁ γ_pub pub ∗
+    inf_chaselev_deque_pub₁ γ_pub pub ∗
     (* state *)
-    inf_chaselev_state γ_lock front back pub.
-  Definition inf_chaselev_inv t : iProp Σ :=
+    inf_chaselev_deque_state γ_lock front back pub.
+  Definition inf_chaselev_deque_inv t : iProp Σ :=
     ∃ l γ_ctl γ_front γ_hist γ_pub γ_lock arr,
     ⌜t = #l⌝ ∗
     (* metas *)
-    meta l inf_chaselev_meta_ctl γ_ctl ∗
-    meta l inf_chaselev_meta_front γ_front ∗
-    meta l inf_chaselev_meta_hist γ_hist ∗
-    meta l inf_chaselev_meta_pub γ_pub ∗
-    meta l inf_chaselev_meta_lock γ_lock ∗
+    meta l inf_chaselev_deque_meta_ctl γ_ctl ∗
+    meta l inf_chaselev_deque_meta_front γ_front ∗
+    meta l inf_chaselev_deque_meta_hist γ_hist ∗
+    meta l inf_chaselev_deque_meta_pub γ_pub ∗
+    meta l inf_chaselev_deque_meta_lock γ_lock ∗
     (* physical fields *)
     l.(array) ↦□ arr ∗
     (* invariant *)
-    inv inf_chaselev_namespace (inf_chaselev_inv_inner l γ_ctl γ_front γ_hist γ_pub γ_lock arr).
+    inv inf_chaselev_deque_namespace (inf_chaselev_deque_inv_inner l γ_ctl γ_front γ_hist γ_pub γ_lock arr).
 
-  Definition inf_chaselev_model t pub : iProp Σ :=
+  Definition inf_chaselev_deque_model t pub : iProp Σ :=
     ∃ l γ_pub,
     ⌜t = #l⌝ ∗
     (* metas *)
-    meta l inf_chaselev_meta_pub γ_pub ∗
+    meta l inf_chaselev_deque_meta_pub γ_pub ∗
     (* public values *)
-    inf_chaselev_pub₂ γ_pub pub.
+    inf_chaselev_deque_pub₂ γ_pub pub.
 
-  Definition inf_chaselev_own t : iProp Σ :=
+  Definition inf_chaselev_deque_own t : iProp Σ :=
     ∃ l γ_ctl γ_lock back priv,
     ⌜t = #l⌝ ∗
     (* metas *)
-    meta l inf_chaselev_meta_ctl γ_ctl ∗
-    meta l inf_chaselev_meta_lock γ_lock ∗
+    meta l inf_chaselev_deque_meta_ctl γ_ctl ∗
+    meta l inf_chaselev_deque_meta_lock γ_lock ∗
     (* control token *)
-    inf_chaselev_ctl₂ γ_ctl back priv ∗
+    inf_chaselev_deque_ctl₂ γ_ctl back priv ∗
     (* lock *)
-    inf_chaselev_lock γ_lock.
+    inf_chaselev_deque_lock γ_lock.
 
-  #[global] Instance inf_chaselev_inv_persistent t :
-    Persistent (inf_chaselev_inv t).
+  #[global] Instance inf_chaselev_deque_inv_persistent t :
+    Persistent (inf_chaselev_deque_inv t).
   Proof.
     apply _.
   Qed.
-  #[global] Instance inf_chaselev_model_timeless t pub :
-    Timeless (inf_chaselev_model t pub).
+  #[global] Instance inf_chaselev_deque_model_timeless t pub :
+    Timeless (inf_chaselev_deque_model t pub).
   Proof.
     apply _.
   Qed.
-  #[global] Instance inf_chaselev_own_timeless t :
-    Timeless (inf_chaselev_own t).
+  #[global] Instance inf_chaselev_deque_own_timeless t :
+    Timeless (inf_chaselev_deque_own t).
   Proof.
     apply _.
   Qed.
 
-  #[local] Lemma inf_chaselev_ctl_alloc :
+  #[local] Lemma inf_chaselev_deque_ctl_alloc :
     ⊢ |==> ∃ γ_ctl,
-      inf_chaselev_ctl₁ γ_ctl 0 (λ _, #()) ∗
-      inf_chaselev_ctl₂ γ_ctl 0 (λ _, #()).
+      inf_chaselev_deque_ctl₁ γ_ctl 0 (λ _, #()) ∗
+      inf_chaselev_deque_ctl₂ γ_ctl 0 (λ _, #()).
   Proof.
     iMod (auth_excl_alloc' ((0%Z, λ _, #()) : prodO ZO (nat -d> valO))) as "(%γ_ctl & Hctl₁ & Hctl₂)".
     iExists γ_ctl. iFrame. done.
   Qed.
-  #[local] Lemma inf_chaselev_ctl_agree γ_ctl back1 priv1 back2 priv2 :
-    inf_chaselev_ctl₁ γ_ctl back1 priv1 -∗
-    inf_chaselev_ctl₂ γ_ctl back2 priv2 -∗
+  #[local] Lemma inf_chaselev_deque_ctl_agree γ_ctl back1 priv1 back2 priv2 :
+    inf_chaselev_deque_ctl₁ γ_ctl back1 priv1 -∗
+    inf_chaselev_deque_ctl₂ γ_ctl back2 priv2 -∗
     ⌜back1 = back2 ∧ priv1 = priv2⌝.
   Proof.
     iIntros "Hctl₁ Hctl₂".
     iDestruct (auth_excl_both_agree with "Hctl₁ Hctl₂") as %(? & ?%functional_extensionality).
     done.
   Qed.
-  #[local] Lemma inf_chaselev_ctl_update {γ_ctl back1 priv1 back2 priv2} back priv :
-    inf_chaselev_ctl₁ γ_ctl back1 priv1 -∗
-    inf_chaselev_ctl₂ γ_ctl back2 priv2 ==∗
-      inf_chaselev_ctl₁ γ_ctl back priv ∗
-      inf_chaselev_ctl₂ γ_ctl back priv.
+  #[local] Lemma inf_chaselev_deque_ctl_update {γ_ctl back1 priv1 back2 priv2} back priv :
+    inf_chaselev_deque_ctl₁ γ_ctl back1 priv1 -∗
+    inf_chaselev_deque_ctl₂ γ_ctl back2 priv2 ==∗
+      inf_chaselev_deque_ctl₁ γ_ctl back priv ∗
+      inf_chaselev_deque_ctl₂ γ_ctl back priv.
   Proof.
     iIntros "Hctl₁ Hctl₂".
     iMod (auth_excl_update' with "Hctl₁ Hctl₂") as "(Hctl₁ & Hctl2)".
     iFrame. done.
   Qed.
 
-  #[local] Lemma inf_chaselev_front_alloc :
+  #[local] Lemma inf_chaselev_deque_front_alloc :
     ⊢ |==> ∃ γ_front,
-      inf_chaselev_front_auth γ_front 0.
+      inf_chaselev_deque_front_auth γ_front 0.
   Proof.
     iMod (auth_nat_max_alloc 0) as "(%γ_front & Hfront_auth & _)".
     iExists γ_front. done.
   Qed.
-  #[local] Lemma inf_chaselev_front_valid γ_front front1 front2 :
-    inf_chaselev_front_auth γ_front front1 -∗
-    inf_chaselev_front_frag γ_front front2 -∗
+  #[local] Lemma inf_chaselev_deque_front_valid γ_front front1 front2 :
+    inf_chaselev_deque_front_auth γ_front front1 -∗
+    inf_chaselev_deque_front_frag γ_front front2 -∗
     ⌜front2 ≤ front1⌝.
   Proof.
     iApply auth_nat_max_both_valid.
   Qed.
-  #[local] Lemma inf_chaselev_front_auth_update {γ_front front} front' :
+  #[local] Lemma inf_chaselev_deque_front_auth_update {γ_front front} front' :
     front ≤ front' →
-    inf_chaselev_front_auth γ_front front ==∗
-    inf_chaselev_front_auth γ_front front'.
+    inf_chaselev_deque_front_auth γ_front front ==∗
+    inf_chaselev_deque_front_auth γ_front front'.
   Proof.
     intros. iApply auth_nat_max_update. done.
   Qed.
-  #[local] Lemma inf_chaselev_front_frag_get γ_front front :
-    inf_chaselev_front_auth γ_front front -∗
-    inf_chaselev_front_frag γ_front front.
+  #[local] Lemma inf_chaselev_deque_front_frag_get γ_front front :
+    inf_chaselev_deque_front_auth γ_front front -∗
+    inf_chaselev_deque_front_frag γ_front front.
   Proof.
     iApply auth_nat_max_frag_get.
   Qed.
 
   (* TODO: hist lemmas *)
-  #[local] Lemma inf_chaselev_hist_alloc :
+  #[local] Lemma inf_chaselev_deque_hist_alloc :
     ⊢ |==> ∃ γ_hist,
-      inf_chaselev_hist_auth γ_hist [] [].
+      inf_chaselev_deque_hist_auth γ_hist [] [].
   Proof.
     iMod (mono_list_own_alloc []) as "(%γ_hist & Hhist_auth & _)".
     iExists γ_hist. done.
   Qed.
 
-  #[local] Lemma inf_chaselev_pub_alloc :
+  #[local] Lemma inf_chaselev_deque_pub_alloc :
     ⊢ |==> ∃ γ_pub,
-      inf_chaselev_pub₁ γ_pub [] ∗
-      inf_chaselev_pub₂ γ_pub [].
+      inf_chaselev_deque_pub₁ γ_pub [] ∗
+      inf_chaselev_deque_pub₂ γ_pub [].
   Proof.
     iMod (auth_excl_alloc' []) as "(%γ_pub & Hpub₁ & Hpub₂)".
     iExists γ_pub. iFrame. done.
   Qed.
-  #[local] Lemma inf_chaselev_pub_agree γ_pub pub1 pub2 :
-    inf_chaselev_pub₁ γ_pub pub1 -∗
-    inf_chaselev_pub₂ γ_pub pub2 -∗
+  #[local] Lemma inf_chaselev_deque_pub_agree γ_pub pub1 pub2 :
+    inf_chaselev_deque_pub₁ γ_pub pub1 -∗
+    inf_chaselev_deque_pub₂ γ_pub pub2 -∗
     ⌜pub1 = pub2⌝.
   Proof.
     iIntros "Hpub₁ Hpub₂".
     iDestruct (auth_excl_both_agree_L with "Hpub₂ Hpub₁") as %->. done.
   Qed.
-  #[local] Lemma inf_chaselev_pub_update {γ_pub pub1 pub2} pub :
-    inf_chaselev_pub₁ γ_pub pub1 -∗
-    inf_chaselev_pub₂ γ_pub pub2 ==∗
-      inf_chaselev_pub₁ γ_pub pub ∗
-      inf_chaselev_pub₂ γ_pub pub.
+  #[local] Lemma inf_chaselev_deque_pub_update {γ_pub pub1 pub2} pub :
+    inf_chaselev_deque_pub₁ γ_pub pub1 -∗
+    inf_chaselev_deque_pub₂ γ_pub pub2 ==∗
+      inf_chaselev_deque_pub₁ γ_pub pub ∗
+      inf_chaselev_deque_pub₂ γ_pub pub.
   Proof.
     iIntros "Hpub₁ Hpub₂".
     iMod (auth_excl_update' with "Hpub₂ Hpub₁") as "(Hpub₂ & Hpub₁)".
     iFrame. done.
   Qed.
 
-  #[local] Lemma inf_chaselev_lock_alloc :
+  #[local] Lemma inf_chaselev_deque_lock_alloc :
     ⊢ |==> ∃ γ_lock,
-      inf_chaselev_lock γ_lock.
+      inf_chaselev_deque_lock γ_lock.
   Proof.
     apply excl_alloc.
   Qed.
-  #[local] Lemma inf_chaselev_lock_exclusive γ_lock :
-    inf_chaselev_lock γ_lock -∗
-    inf_chaselev_lock γ_lock -∗
+  #[local] Lemma inf_chaselev_deque_lock_exclusive γ_lock :
+    inf_chaselev_deque_lock γ_lock -∗
+    inf_chaselev_deque_lock γ_lock -∗
     False.
   Proof.
     apply excl_exclusive.
   Qed.
-  #[local] Lemma inf_chaselev_lock_state γ_lock front back pub :
-    inf_chaselev_lock γ_lock -∗
-    inf_chaselev_state γ_lock front back pub -∗
-    inf_chaselev_state₁ front back pub.
+  #[local] Lemma inf_chaselev_deque_lock_state γ_lock front back pub :
+    inf_chaselev_deque_lock γ_lock -∗
+    inf_chaselev_deque_state γ_lock front back pub -∗
+    inf_chaselev_deque_state₁ front back pub.
   Proof.
     iIntros "Hlock [Hstate | (Hlock' & Hstate)]"; first done.
-    iDestruct (inf_chaselev_lock_exclusive with "Hlock Hlock'") as %[].
+    iDestruct (inf_chaselev_deque_lock_exclusive with "Hlock Hlock'") as %[].
   Qed.
 
-  Lemma inf_chaselev_own_exclusive t :
-    inf_chaselev_own t -∗
-    inf_chaselev_own t -∗
+  Lemma inf_chaselev_deque_own_exclusive t :
+    inf_chaselev_deque_own t -∗
+    inf_chaselev_deque_own t -∗
     False.
   Proof.
     iIntros "(%l1 & %γ_ctl1 & %γ_lock1 & %back1 & %priv1 & %Heq1 & #Hmeta_ctl1 & #Hmeta_lock1 & Hctl₂1 & Hlock1) (%l2 & %γ_ctl2 & %γ_lock2 & %back2 & %priv2 & %Heq2 & #Hmeta_ctl2 & #Hmeta_lock2 & Hctl₂2 & Hlock2)". simplify.
     iDestruct (meta_agree with "Hmeta_lock1 Hmeta_lock2") as %->.
-    iApply (inf_chaselev_lock_exclusive with "Hlock1 Hlock2").
+    iApply (inf_chaselev_deque_lock_exclusive with "Hlock1 Hlock2").
   Qed.
 
-  Lemma inf_chaselev_make_spec :
+  Lemma inf_chaselev_deque_make_spec :
     {{{ True }}}
-      inf_chaselev_make #()
+      inf_chaselev_deque_make #()
     {{{ t,
       RET t;
-      inf_chaselev_inv t ∗ inf_chaselev_model t [] ∗ inf_chaselev_own t
+      inf_chaselev_deque_inv t ∗ inf_chaselev_deque_model t [] ∗ inf_chaselev_deque_own t
     }}}.
   Proof.
     iIntros "%Φ _ HΦ".
@@ -399,16 +399,16 @@ Section inf_chaselev_GS.
     wp_pures. wp_store.
     iMod (mapsto_persist with "Harr") as "#Harr".
     iApply "HΦ".
-    iMod inf_chaselev_ctl_alloc as "(%γ_ctl & Hctl₁ & Hctl₂)".
-    iMod inf_chaselev_front_alloc as "(%γ_front & Hfront_auth)".
-    iMod inf_chaselev_hist_alloc as "(%γ_hist & Hhist_auth)".
-    iMod inf_chaselev_pub_alloc as "(%γ_pub & Hpub₁ & Hpub₂)".
-    iMod inf_chaselev_lock_alloc as "(%γ_lock & Hlock)".
-    iDestruct (meta_token_difference _ (↑ inf_chaselev_meta_ctl) with "Hmeta") as "(Hmeta_ctl & Hmeta)"; first solve_ndisj.
-    iDestruct (meta_token_difference _ (↑ inf_chaselev_meta_front) with "Hmeta") as "(Hmeta_front & Hmeta)"; first solve_ndisj.
-    iDestruct (meta_token_difference _ (↑ inf_chaselev_meta_hist) with "Hmeta") as "(Hmeta_hist & Hmeta)"; first solve_ndisj.
-    iDestruct (meta_token_difference _ (↑ inf_chaselev_meta_pub) with "Hmeta") as "(Hmeta_pub & Hmeta)"; first solve_ndisj.
-    iDestruct (meta_token_difference _ (↑ inf_chaselev_meta_lock) with "Hmeta") as "(Hmeta_lock & Hmeta)"; first solve_ndisj.
+    iMod inf_chaselev_deque_ctl_alloc as "(%γ_ctl & Hctl₁ & Hctl₂)".
+    iMod inf_chaselev_deque_front_alloc as "(%γ_front & Hfront_auth)".
+    iMod inf_chaselev_deque_hist_alloc as "(%γ_hist & Hhist_auth)".
+    iMod inf_chaselev_deque_pub_alloc as "(%γ_pub & Hpub₁ & Hpub₂)".
+    iMod inf_chaselev_deque_lock_alloc as "(%γ_lock & Hlock)".
+    iDestruct (meta_token_difference _ (↑ inf_chaselev_deque_meta_ctl) with "Hmeta") as "(Hmeta_ctl & Hmeta)"; first solve_ndisj.
+    iDestruct (meta_token_difference _ (↑ inf_chaselev_deque_meta_front) with "Hmeta") as "(Hmeta_front & Hmeta)"; first solve_ndisj.
+    iDestruct (meta_token_difference _ (↑ inf_chaselev_deque_meta_hist) with "Hmeta") as "(Hmeta_hist & Hmeta)"; first solve_ndisj.
+    iDestruct (meta_token_difference _ (↑ inf_chaselev_deque_meta_pub) with "Hmeta") as "(Hmeta_pub & Hmeta)"; first solve_ndisj.
+    iDestruct (meta_token_difference _ (↑ inf_chaselev_deque_meta_lock) with "Hmeta") as "(Hmeta_lock & Hmeta)"; first solve_ndisj.
     iMod (meta_set _ _ γ_ctl with "Hmeta_ctl") as "#Hmeta_ctl"; first done.
     iMod (meta_set _ _ γ_front with "Hmeta_front") as "#Hmeta_front"; first done.
     iMod (meta_set _ _ γ_hist with "Hmeta_hist") as "#Hmeta_hist"; first done.
@@ -425,16 +425,16 @@ Section inf_chaselev_GS.
     iExists l, γ_ctl, γ_lock, 0%Z, (λ _, #()). iFrame "∗#". done.
   Qed.
 
-  Lemma inf_chaselev_push_spec t v :
+  Lemma inf_chaselev_deque_push_spec t v :
     <<<
-      inf_chaselev_inv t ∗ inf_chaselev_own t |
-      ∀∀ pub, inf_chaselev_model t pub
+      inf_chaselev_deque_inv t ∗ inf_chaselev_deque_own t |
+      ∀∀ pub, inf_chaselev_deque_model t pub
     >>>
-      inf_chaselev_push t v
-      @ ↑ inf_chaselev_namespace
+      inf_chaselev_deque_push t v
+      @ ↑ inf_chaselev_deque_namespace
     <<<
-      inf_chaselev_model t (pub ++ [v]) |
-      RET #(); inf_chaselev_own t
+      inf_chaselev_deque_model t (pub ++ [v]) |
+      RET #(); inf_chaselev_deque_own t
     >>>.
   Proof.
     iIntros "!> %Φ ((%l & %γ_ctl & %γ_front & %γ_hist & %γ_pub & %γ_lock & %arr & -> & #Hmeta_ctl & #Hmeta_front & #Hmeta_hist & #Hmeta_pub & #Hmeta_lock & #Harr & #Hinv) & (%l' & %_γ_ctl & %_γ_lock & %back & %priv & %Heq & #_Hmeta_ctl & #_Hmeta_lock & Hctl₂ & Hlock)) HΦ".
@@ -448,11 +448,11 @@ Section inf_chaselev_GS.
     wp_bind (!#l.(back))%E.
     (* open invariant *)
     iInv "Hinv" as "(%front & %_back & %hist & %pub & %_priv & Hfront & Hback & >Hctl₁ & Hfront_auth & Harr_model & >%Hhist & Hhist_auth & Hpub₁ & Hstate)".
-    iDestruct (inf_chaselev_ctl_agree with "Hctl₁ Hctl₂") as %?. simplify- front.
+    iDestruct (inf_chaselev_deque_ctl_agree with "Hctl₁ Hctl₂") as %?. simplify- front.
     (* do load [back] *)
     wp_load.
     (* we have lock, hence we are in state 1 *)
-    iDestruct (inf_chaselev_lock_state with "Hlock Hstate") as %Hstate.
+    iDestruct (inf_chaselev_deque_lock_state with "Hlock Hstate") as %Hstate.
     (* hence, [0 ≤ back] *)
     assert (0 ≤ back)%Z as Hback by lia.
     (* close invariant *)
@@ -471,14 +471,14 @@ Section inf_chaselev_GS.
     awp_apply (inf_array_set_spec with "[//]") without "HΦ"; first done.
     (* open invariant *)
     iInv "Hinv" as "(%front & %_back & %hist & %pub & %_priv & Hfront & Hback & >Hctl₁ & Hfront_auth & >Harr_model & >%Hhist & Hhist_auth & Hpub₁ & >Hstate)".
-    iDestruct (inf_chaselev_ctl_agree with "Hctl₁ Hctl₂") as %?. simplify- front.
+    iDestruct (inf_chaselev_deque_ctl_agree with "Hctl₁ Hctl₂") as %?. simplify- front.
     iAaccIntro with "Harr_model"; iIntros "Harr_model".
     { iModIntro. iFrame. repeat iExists _. iFrame. done. }
     (* update [priv] in control tokens *)
     set (priv' := <[0 := v]> priv).
-    iMod (inf_chaselev_ctl_update back priv' with "Hctl₁ Hctl₂") as "(Hctl₁ & Hctl₂)".
+    iMod (inf_chaselev_deque_ctl_update back priv' with "Hctl₁ Hctl₂") as "(Hctl₁ & Hctl₂)".
     (* we have lock, hence we are in state 1 *)
-    iDestruct (inf_chaselev_lock_state with "Hlock Hstate") as %(Hstate & Hpub).
+    iDestruct (inf_chaselev_deque_lock_state with "Hlock Hstate") as %(Hstate & Hpub).
     (* close invariant *)
     iModIntro. iSplitL "Hfront Hback Hctl₁ Hfront_auth Harr_model Hhist_auth Hpub₁ Hstate".
     { iNext. iExists front, back, hist, pub, priv'. iFrame. iSplit; last done.
@@ -503,30 +503,30 @@ Section inf_chaselev_GS.
     (* → [#l.(back) <- #(back + 1)] *)
     (* open invariant *)
     iInv "Hinv" as "(%front & %_back & %hist & %pub & %_priv & Hfront & Hback & >Hctl₁ & Hfront_auth & Harr_model & >%Hhist & Hhist_auth & Hpub₁ & Hstate)".
-    iDestruct (inf_chaselev_ctl_agree with "Hctl₁ Hctl₂") as %?. simplify- front.
+    iDestruct (inf_chaselev_deque_ctl_agree with "Hctl₁ Hctl₂") as %?. simplify- front.
     (* do increment [back] *)
     wp_store.
     (* update [priv] in control tokens *)
     set (priv'' := λ i, priv (S i)).
-    iMod (inf_chaselev_ctl_update (back + 1) priv'' with "Hctl₁ Hctl₂") as "(Hctl₁ & Hctl₂)".
+    iMod (inf_chaselev_deque_ctl_update (back + 1) priv'' with "Hctl₁ Hctl₂") as "(Hctl₁ & Hctl₂)".
     (* begin transaction *)
     iMod "HΦ" as "(%_pub & (%_l & %_γ_pub & %Heq & _Hmeta_pub & Hpub₂) & _ & HΦ)".
     injection Heq as <-.
     iDestruct (meta_agree with "Hmeta_pub _Hmeta_pub") as %<-. iClear "_Hmeta_pub".
-    iDestruct (inf_chaselev_pub_agree with "Hpub₁ Hpub₂") as %<-.
+    iDestruct (inf_chaselev_deque_pub_agree with "Hpub₁ Hpub₂") as %<-.
     (* update [pub] *)
     set (pub' := pub ++ [v]).
-    iMod (inf_chaselev_pub_update pub' with "Hpub₁ Hpub₂") as "(Hpub₁ & Hpub₂)".
+    iMod (inf_chaselev_deque_pub_update pub' with "Hpub₁ Hpub₂") as "(Hpub₁ & Hpub₂)".
     (* end transaction *)
     iMod ("HΦ" with "[Hpub₂]") as "HΦ".
     { iExists l, γ_pub. iFrame "∗#". done. }
     (* update [hist] *)
-    iAssert (inf_chaselev_hist_auth γ_hist hist pub')%I with "[>Hhist_auth]" as "Hhist_auth".
+    iAssert (inf_chaselev_deque_hist_auth γ_hist hist pub')%I with "[>Hhist_auth]" as "Hhist_auth".
     { destruct pub; last done.
       iMod (mono_list_auth_own_update_app [v] with "Hhist_auth") as "($ & _)". done.
     }
     (* we have lock, hence we are in state 1 *)
-    iDestruct (inf_chaselev_lock_state with "Hlock Hstate") as %(Hstate & Hpub).
+    iDestruct (inf_chaselev_deque_lock_state with "Hlock Hstate") as %(Hstate & Hpub).
     (* close invariant *)
     iModIntro. iSplitL "Hfront Hback Hctl₁ Hfront_auth Harr_model Hhist_auth Hpub₁ Hstate".
     { iNext. iExists front, (back + 1)%Z, hist, pub', priv''. iFrame.
@@ -555,17 +555,17 @@ Section inf_chaselev_GS.
     iApply "HΦ". repeat iExists _. iFrame "∗#". done.
   Qed.
 
-  Lemma inf_chaselev_steal_spec t :
+  Lemma inf_chaselev_deque_steal_spec t :
     <<<
-      inf_chaselev_inv t |
-      ∀∀ pub, inf_chaselev_model t pub
+      inf_chaselev_deque_inv t |
+      ∀∀ pub, inf_chaselev_deque_model t pub
     >>>
-      inf_chaselev_steal t
-      @ ↑ inf_chaselev_namespace
+      inf_chaselev_deque_steal t
+      @ ↑ inf_chaselev_deque_namespace
     <<<
       ∃∃ o,
-      (⌜length pub ≤ 1 ∧ o = NONEV⌝ ∗ inf_chaselev_model t pub) ∨
-      (∃ pub' v, ⌜pub = v :: pub' ∧ o = SOMEV v⌝ ∗ inf_chaselev_model t pub') |
+      (⌜length pub ≤ 1 ∧ o = NONEV⌝ ∗ inf_chaselev_deque_model t pub) ∨
+      (∃ pub' v, ⌜pub = v :: pub' ∧ o = SOMEV v⌝ ∗ inf_chaselev_deque_model t pub') |
       RET o; True
     >>>.
   Proof.
@@ -580,7 +580,7 @@ Section inf_chaselev_GS.
     iInv "Hinv" as "(%front1 & %back1 & %hist & %pub & %priv & Hfront & Hback & Hctl₁ & Hfront_auth & Harr_model & >%Hhist & Hhist_auth & Hpub₁ & Hstate)".
     wp_load.
     (* emit front fragment at [front1] *)
-    iDestruct (inf_chaselev_front_frag_get with "Hfront_auth") as "#Hfront_frag".
+    iDestruct (inf_chaselev_deque_front_frag_get with "Hfront_auth") as "#Hfront_frag".
     (* close invariant *)
     iModIntro. iSplitL "Hfront Hback Hctl₁ Hfront_auth Harr_model Hhist_auth Hpub₁ Hstate".
     { repeat iExists _. iFrame. done. }
@@ -598,7 +598,7 @@ Section inf_chaselev_GS.
     { (* we have [1 ≤ length pub] *)
       iAssert ⌜length pub ≤ 1⌝%I as %Hpub.
       { iDestruct "Hstate" as "[%Hstate | (Hlock & [%Hstate | %Hstate])]".
-        - iDestruct (inf_chaselev_front_valid with "Hfront_auth Hfront_frag") as %?.
+        - iDestruct (inf_chaselev_deque_front_valid with "Hfront_auth Hfront_frag") as %?.
           destruct (decide (back2 = front1)) as [-> |]; last lia.
           assert (front1 = front2) as <- by lia. iPureIntro. lia.
         - iPureIntro. lia.
@@ -607,7 +607,7 @@ Section inf_chaselev_GS.
       (* begin transaction *)
       iMod "HΦ" as "(%_pub & (%_l & %_γ_pub & %Heq & #_Hmeta_pub & Hpub₂) & _ & HΦ)". injection Heq as <-.
       iDestruct (meta_agree with "Hmeta_pub _Hmeta_pub") as %<-. iClear "_Hmeta_pub".
-      iDestruct (inf_chaselev_pub_agree with "Hpub₁ Hpub₂") as %<-.
+      iDestruct (inf_chaselev_deque_pub_agree with "Hpub₁ Hpub₂") as %<-.
       (* end transation *)
       iMod ("HΦ" with "[Hpub₂] [//]") as "HΦ".
       { iLeft. iSplit; first done. repeat iExists _. naive_solver. }
@@ -631,12 +631,12 @@ Section inf_chaselev_GS.
       iApply "HΦ".
     }
     (* we have [front1 ≤ front2] *)
-    iDestruct (inf_chaselev_front_valid with "Hfront_auth Hfront_frag") as %Hbr2.
+    iDestruct (inf_chaselev_deque_front_valid with "Hfront_auth Hfront_frag") as %Hbr2.
     (* enforce [front2 = front1] *)
     rewrite Nat.le_lteq in Hbr2. destruct Hbr2 as [Hbr2 | <-].
     { (* emit front fragment at [front2] *)
       iClear "Hfront_frag".
-      iDestruct (inf_chaselev_front_frag_get with "Hfront_auth") as "#Hfront_frag".
+      iDestruct (inf_chaselev_deque_front_frag_get with "Hfront_auth") as "#Hfront_frag".
       (* close invariant *)
       iModIntro. iSplitL "Hfront Hback Hctl₁ Hfront_auth Harr_model Hhist_auth Hpub₁ Hstate".
       { repeat iExists _. iFrame. done. }
@@ -676,7 +676,7 @@ Section inf_chaselev_GS.
       (* CAS must fail as we have seen [front2] such that [front1 < front2] *)
       wp_cmpxchg as ? | _.
       { simplify- front1.
-        iDestruct (inf_chaselev_front_valid with "Hfront_auth Hfront_frag") as %?.
+        iDestruct (inf_chaselev_deque_front_valid with "Hfront_auth Hfront_frag") as %?.
         lia.
       }
       (* close invariant *)
@@ -685,7 +685,7 @@ Section inf_chaselev_GS.
 
       wp_pures.
 
-      (* → [inf_chaselev_steal #l] *)
+      (* → [inf_chaselev_deque_steal #l] *)
       wp_apply ("HLöb" with "HΦ").
     }
     (* we are in state 1, hence [length pub = back2 - front1] *)
@@ -694,7 +694,7 @@ Section inf_chaselev_GS.
     (* hence, [pub] contains at least one value *)
     destruct pub as [| v pub]; first naive_solver lia.
     (* emit history fragment at [front1] *)
-    iAssert (inf_chaselev_hist_frag γ_hist front1 v) as "#Hhist_frag".
+    iAssert (inf_chaselev_deque_hist_frag γ_hist front1 v) as "#Hhist_frag".
     { iDestruct (mono_list_lb_own_get with "Hhist_auth") as "#Hhist_frag".
       iApply (mono_list_idx_own_get with "Hhist_frag").
       rewrite lookup_app_r; last lia.
@@ -724,12 +724,12 @@ Section inf_chaselev_GS.
     iAaccIntro with "Harr_model"; iIntros "Harr_model".
     { iModIntro. rewrite right_id. repeat iExists _. iFrame. done. }
     (* we have [front1 < front3] *)
-    iDestruct (inf_chaselev_front_valid with "Hfront_auth Hfront_frag") as %Hbr3.
+    iDestruct (inf_chaselev_deque_front_valid with "Hfront_auth Hfront_frag") as %Hbr3.
     (* enforce [front3 = front1] *)
     rewrite Nat.le_lteq in Hbr3. destruct Hbr3 as [Hbr3 | <-].
     { (* emit front fragment at [front3] *)
       iClear "Hfront_frag".
-      iDestruct (inf_chaselev_front_frag_get with "Hfront_auth") as "#Hfront_frag".
+      iDestruct (inf_chaselev_deque_front_frag_get with "Hfront_auth") as "#Hfront_frag".
       (* close invariant *)
       iModIntro. iSplitL "Hfront Hback Hctl₁ Hfront_auth Harr_model Hhist_auth Hpub₁ Hstate".
       { repeat iExists _. iFrame. done. }
@@ -746,7 +746,7 @@ Section inf_chaselev_GS.
       (* CAS must fail as we have seen [front3] such that [front1 < front3] *)
       wp_cmpxchg as ? | _.
       { simplify- front1.
-        iDestruct (inf_chaselev_front_valid with "Hfront_auth Hfront_frag") as %?.
+        iDestruct (inf_chaselev_deque_front_valid with "Hfront_auth Hfront_frag") as %?.
         lia.
       }
       (* close invariant *)
@@ -755,7 +755,7 @@ Section inf_chaselev_GS.
 
       wp_pures.
 
-      (* → [inf_chaselev_steal #l] *)
+      (* → [inf_chaselev_deque_steal #l] *)
       wp_apply ("HLöb" with "HΦ").
     }
     (* from history fragment at [front1], we know the loaded value is [v] *)
@@ -793,14 +793,14 @@ Section inf_chaselev_GS.
 
       wp_pures.
 
-      (* → [inf_chaselev_steal #l] *)
+      (* → [inf_chaselev_deque_steal #l] *)
       wp_apply ("HLöb" with "HΦ").
     }
     simplify- front1.
     iDestruct "Hmodel" as "(%_l & %_γ_pub & %Heq & #_Hmeta_pub & Hpub₂)".
     injection Heq as <-.
     iDestruct (meta_agree with "Hmeta_pub _Hmeta_pub") as %<-. iClear "_Hmeta_pub".
-    iDestruct (inf_chaselev_pub_agree with "Hpub₁ Hpub₂") as %<-.
+    iDestruct (inf_chaselev_deque_pub_agree with "Hpub₁ Hpub₂") as %<-.
     (* [front] has not changed, hence [v] is still the front public value *)
     iDestruct (mono_list_auth_idx_lookup with "Hhist_auth Hhist_frag") as %Hhist_lookup.
     destruct pub as [| w pub].
@@ -808,19 +808,19 @@ Section inf_chaselev_GS.
     rewrite lookup_app_r in Hhist_lookup; last lia.
     apply list_lookup_singleton_Some in Hhist_lookup as (_ & ->).
     (* end transation *)
-    iMod (inf_chaselev_pub_update pub with "Hpub₁ Hpub₂") as "(Hpub₁ & Hpub₂)".
-    iAssert (inf_chaselev_model #l pub) with "[Hpub₂]" as "Hmodel".
+    iMod (inf_chaselev_deque_pub_update pub with "Hpub₁ Hpub₂") as "(Hpub₁ & Hpub₂)".
+    iAssert (inf_chaselev_deque_model #l pub) with "[Hpub₂]" as "Hmodel".
     { iExists l, γ_pub. naive_solver. }
     iMod ("HΦ" with "[Hmodel] [//]") as "HΦ"; first eauto. iModIntro.
     (* update front authority *)
-    iMod (inf_chaselev_front_auth_update (S front1) with "Hfront_auth") as "Hfront_auth"; first lia.
+    iMod (inf_chaselev_deque_front_auth_update (S front1) with "Hfront_auth") as "Hfront_auth"; first lia.
     (* update [hist] *)
-    iAssert (inf_chaselev_hist_auth γ_hist (hist ++ [v]) pub) with "[> Hhist_auth]" as "Hhist_auth".
+    iAssert (inf_chaselev_deque_hist_auth γ_hist (hist ++ [v]) pub) with "[> Hhist_auth]" as "Hhist_auth".
     { destruct pub as [| w pub]; first done.
       iMod (mono_list_auth_own_update_app with "Hhist_auth") as "($ & _)". done.
     }
     (* update state *)
-    iAssert (inf_chaselev_state γ_lock (S front1) back4 pub) with "[Hstate]" as "Hstate".
+    iAssert (inf_chaselev_deque_state γ_lock (S front1) back4 pub) with "[Hstate]" as "Hstate".
     { iDestruct "Hstate" as "[%Hstate | (Hlock & [%Hstate | %Hstate])]".
       - iLeft. naive_solver auto with lia.
       - iRight. iFrame. iRight. iPureIntro.
@@ -847,18 +847,18 @@ Section inf_chaselev_GS.
     iApply "HΦ".
   Qed.
 
-  Lemma inf_chaselev_pop_spec t :
+  Lemma inf_chaselev_deque_pop_spec t :
     <<<
-      inf_chaselev_inv t ∗ inf_chaselev_own t |
-      ∀∀ pub, inf_chaselev_model t pub
+      inf_chaselev_deque_inv t ∗ inf_chaselev_deque_own t |
+      ∀∀ pub, inf_chaselev_deque_model t pub
     >>>
-      inf_chaselev_pop t
-      @ ↑ inf_chaselev_namespace
+      inf_chaselev_deque_pop t
+      @ ↑ inf_chaselev_deque_namespace
     <<<
       ∃∃ o,
-      (⌜pub = [] ∧ o = NONEV⌝ ∗ inf_chaselev_model t []) ∨
-      (∃ pub' v, ⌜pub = pub' ++ [v] ∧ o = SOMEV v⌝ ∗ inf_chaselev_model t pub') |
-      RET o; inf_chaselev_own t
+      (⌜pub = [] ∧ o = NONEV⌝ ∗ inf_chaselev_deque_model t []) ∨
+      (∃ pub' v, ⌜pub = pub' ++ [v] ∧ o = SOMEV v⌝ ∗ inf_chaselev_deque_model t pub') |
+      RET o; inf_chaselev_deque_own t
     >>>.
   Proof.
     iIntros "!> %Φ ((%l & %γ_ctl & %γ_front & %γ_hist & %γ_pub & %γ_lock & %arr & -> & #Hmeta_ctl & #Hmeta_front & #Hmeta_hist & #Hmeta_pub & #Hmeta_lock & #Harr & #Hinv) & (%_l & %_γ_ctl & %_γ_lock & %back & %priv & %Heq & #_Hmeta_ctl & #_Hmeta_lock & Hctl₂ & Hlock)) HΦ".
@@ -873,7 +873,7 @@ Section inf_chaselev_GS.
     wp_bind (!#l.(back))%E.
     (* open invariant *)
     iInv "Hinv" as "(%front1 & %_back & %hist & %pub & %_priv & Hfront & Hback & >Hctl₁ & Hfront_auth & Harr_model & >%Hhist & Hhist_auth & Hpub₁ & Hstate)".
-    iDestruct (inf_chaselev_ctl_agree with "Hctl₁ Hctl₂") as %?. simplify- front1.
+    iDestruct (inf_chaselev_deque_ctl_agree with "Hctl₁ Hctl₂") as %?. simplify- front1.
     (* do load [back] *)
     wp_load.
     (* close invariant *)
@@ -892,13 +892,13 @@ Section inf_chaselev_GS.
     wp_bind (#l.(back) <- #(back - 1))%E.
     (* open invariant *)
     iInv "Hinv" as "(%front2 & %_back & %hist & %pub & %_priv & Hfront & Hback & >Hctl₁ & Hfront_auth & Harr_model & >%Hhist & Hhist_auth & Hpub₁ & Hstate)".
-    iDestruct (inf_chaselev_ctl_agree with "Hctl₁ Hctl₂") as %?. simplify- front2.
+    iDestruct (inf_chaselev_deque_ctl_agree with "Hctl₁ Hctl₂") as %?. simplify- front2.
     (* do decrement [back] *)
     wp_store.
     (* update [back] in control tokens *)
-    iMod (inf_chaselev_ctl_update (back - 1) priv with "Hctl₁ Hctl₂") as "(Hctl₁ & Hctl₂)".
+    iMod (inf_chaselev_deque_ctl_update (back - 1) priv with "Hctl₁ Hctl₂") as "(Hctl₁ & Hctl₂)".
     (* we have lock, hence we are in state 1 *)
-    iDestruct (inf_chaselev_lock_state with "Hlock Hstate") as %(Hstate & Hpub).
+    iDestruct (inf_chaselev_deque_lock_state with "Hlock Hstate") as %(Hstate & Hpub).
     (* branching 1 *)
     destruct (Z.lt_total back (front2 + 1)) as [Hbr1 | [-> | Hbr1]].
 
@@ -906,7 +906,7 @@ Section inf_chaselev_GS.
     - (* we are in state 1, hence [back = front2] *)
       assert (front2 = Z.to_nat back) as -> by lia.
       (* emit front fragment at [back] *)
-      iDestruct (inf_chaselev_front_frag_get with "Hfront_auth") as "#Hfront_frag".
+      iDestruct (inf_chaselev_deque_front_frag_get with "Hfront_auth") as "#Hfront_frag".
       (* close invariant *)
       iModIntro. iSplitL "Hfront Hback Hctl₁ Hfront_auth Harr_model Hhist_auth Hpub₁ Hstate Hlock".
       { iNext. iExists (Z.to_nat back), (back - 1)%Z, hist, pub, priv. iFrame. iSplit; first done.
@@ -921,11 +921,11 @@ Section inf_chaselev_GS.
       wp_bind (!#l.(front))%E.
       (* open invariant *)
       iInv "Hinv" as "(%front3 & %_back & %hist & %pub & %_priv & Hfront & Hback & >Hctl₁ & Hfront_auth & Harr_model & >%Hhist & Hhist_auth & Hpub₁ & Hstate)".
-      iDestruct (inf_chaselev_ctl_agree with "Hctl₁ Hctl₂") as %?. simplify- front3.
+      iDestruct (inf_chaselev_deque_ctl_agree with "Hctl₁ Hctl₂") as %?. simplify- front3.
       (* do load [front] *)
       wp_load.
       (* from front fragment at [back], we know [back ≤ front3] *)
-      iDestruct (inf_chaselev_front_valid with "Hfront_auth Hfront_frag") as %Hfront3.
+      iDestruct (inf_chaselev_deque_front_valid with "Hfront_auth Hfront_frag") as %Hfront3.
       (* hence, we have [back = front3] *)
       iAssert ⌜back = front3⌝%I as %Hstate; last iEval (rewrite -Hstate).
       { iDestruct "Hstate" as "[%Hstate | (Hlock & [%Hstate | %Hstate])]"; auto with lia. }
@@ -945,13 +945,13 @@ Section inf_chaselev_GS.
       wp_bind (#l.(back) <- #back)%E.
       (* open invariant *)
       iInv "Hinv" as "(%front4 & %_back & %hist & %pub & %_priv & Hfront & Hback & >Hctl₁ & Hfront_auth & Harr_model & >%Hhist & Hhist_auth & Hpub₁ & Hstate)".
-      iDestruct (inf_chaselev_ctl_agree with "Hctl₁ Hctl₂") as %?. simplify- front4.
+      iDestruct (inf_chaselev_deque_ctl_agree with "Hctl₁ Hctl₂") as %?. simplify- front4.
       (* do increment [back] *)
       wp_store.
       (* update [back] in control tokens *)
-      iMod (inf_chaselev_ctl_update back priv with "Hctl₁ Hctl₂") as "(Hctl₁ & Hctl₂)".
+      iMod (inf_chaselev_deque_ctl_update back priv with "Hctl₁ Hctl₂") as "(Hctl₁ & Hctl₂)".
       (* from front fragment at [back], we know [back ≤ front4] *)
-      iDestruct (inf_chaselev_front_valid with "Hfront_auth Hfront_frag") as %Hfront4.
+      iDestruct (inf_chaselev_deque_front_valid with "Hfront_auth Hfront_frag") as %Hfront4.
       (* hence, we are in state 2.2 *)
       iDestruct "Hstate" as "[%Hstate | (Hlock & [%Hstate | %Hstate])]"; [lia.. |].
       (* hence, [front4 = back] *)
@@ -959,7 +959,7 @@ Section inf_chaselev_GS.
       (* begin transaction *)
       iMod "HΦ" as "(%_pub & (%_l & %_γ_pub & %Heq & #_Hmeta_pub & Hpub₂) & _ & HΦ)". injection Heq as <-.
       iDestruct (meta_agree with "Hmeta_pub _Hmeta_pub") as %<-.
-      iDestruct (inf_chaselev_pub_agree with "Hpub₁ Hpub₂") as %<-.
+      iDestruct (inf_chaselev_deque_pub_agree with "Hpub₁ Hpub₂") as %<-.
       (* end transaction *)
       iMod ("HΦ" $! NONEV with "[Hpub₂]") as "HΦ".
       { iLeft. simplify. iSplit; first done. repeat iExists _. naive_solver. }
@@ -977,13 +977,13 @@ Section inf_chaselev_GS.
     (* branch 1.2: back = front2 + 1; race for last public value *)
     - assert ((front2 + 1 - 1)%Z = front2) as -> by lia.
       (* emit front fragment at [front2] *)
-      iDestruct (inf_chaselev_front_frag_get with "Hfront_auth") as "#Hfront_frag".
+      iDestruct (inf_chaselev_deque_front_frag_get with "Hfront_auth") as "#Hfront_frag".
       assert (∃ v, pub = [v]) as (v & ->).
       { assert (length pub = 1) by lia.
         destruct pub as [| v pub]; first done. eexists v. destruct pub; done.
       }
       (* emit history fragment at [front2] *)
-      iAssert (inf_chaselev_hist_frag γ_hist front2 v) as "#Hhist_frag".
+      iAssert (inf_chaselev_deque_hist_frag γ_hist front2 v) as "#Hhist_frag".
       { iDestruct (mono_list_lb_own_get with "Hhist_auth") as "#Hhist_frag".
         iApply (mono_list_idx_own_get with "Hhist_frag").
         rewrite lookup_app_r; last lia.
@@ -1002,7 +1002,7 @@ Section inf_chaselev_GS.
       wp_bind (!#l.(front))%E.
       (* open invariant *)
       iInv "Hinv" as "(%front3 & %_back & %hist & %pub & %_priv & Hfront & Hback & >Hctl₁ & Hfront_auth & Harr_model & >%Hhist & Hhist_auth & Hpub₁ & Hstate)".
-      iDestruct (inf_chaselev_ctl_agree with "Hctl₁ Hctl₂") as %?. simplify- front3.
+      iDestruct (inf_chaselev_deque_ctl_agree with "Hctl₁ Hctl₂") as %?. simplify- front3.
       (* do load [front] *)
       wp_load.
       (* branching 2 *)
@@ -1012,7 +1012,7 @@ Section inf_chaselev_GS.
       + (* we have [front3 = front2] *)
         iAssert ⌜front3 = front2⌝%I as %->.
         { (* from front fragment at [front2], we know [front2 ≤ front3] *)
-          iDestruct (inf_chaselev_front_valid with "Hfront_auth Hfront_frag") as %?.
+          iDestruct (inf_chaselev_deque_front_valid with "Hfront_auth Hfront_frag") as %?.
           iPureIntro. lia.
         }
         (* hence, [pub] is empty *)
@@ -1043,7 +1043,7 @@ Section inf_chaselev_GS.
         awp_apply (inf_array_get_spec with "[//]")  without "HΦ"; first lia.
         (* open invariant *)
         iInv "Hinv" as "(%front4 & %_back & %hist & %pub & %_priv & Hfront & Hback & >Hctl₁ & Hfront_auth & >Harr_model & >%Hhist & >Hhist_auth & Hpub₁ & Hstate)".
-        iDestruct (inf_chaselev_ctl_agree with "Hctl₁ Hctl₂") as %?. simplify- front4.
+        iDestruct (inf_chaselev_deque_ctl_agree with "Hctl₁ Hctl₂") as %?. simplify- front4.
         iAaccIntro with "Harr_model"; iIntros "Harr_model".
         { iModIntro. iFrame. iNext. repeat iExists _. iFrame. done. }
         (* from history fragment at [front2], we know [(hist ++ pub) !! front2 = Some v] *)
@@ -1073,7 +1073,7 @@ Section inf_chaselev_GS.
         wp_bind (CmpXchg #l.(front) #front2 #(front2 + 1))%E.
         (* open invariant *)
         iInv "Hinv" as "(%front5 & %_back & %hist & %pub & %_priv & Hfront & Hback & >Hctl₁ & >Hfront_auth & Harr_model & >%Hhist & >Hhist_auth & >Hpub₁ & >Hstate)".
-        iDestruct (inf_chaselev_ctl_agree with "Hctl₁ Hctl₂") as %?. simplify- front5.
+        iDestruct (inf_chaselev_deque_ctl_agree with "Hctl₁ Hctl₂") as %?. simplify- front5.
         (* branch 3 *)
         iDestruct "Hstate" as "[%Hstate | (Hlock & [%Hstate | %Hstate])]".
 
@@ -1081,7 +1081,7 @@ Section inf_chaselev_GS.
         * (* we have [front5 = front2] *)
           iAssert ⌜front5 = front2⌝%I as %->.
           { (* from front fragment at [front2], we know [front2 ≤ front5] *)
-            iDestruct (inf_chaselev_front_valid with "Hfront_auth Hfront_frag") as %?.
+            iDestruct (inf_chaselev_deque_front_valid with "Hfront_auth Hfront_frag") as %?.
             iPureIntro. lia.
           }
           (* hence, [pub] is empty *)
@@ -1106,16 +1106,16 @@ Section inf_chaselev_GS.
           iMod "HΦ" as "(%_pub & (%_l & %_γ_pub & %Heq & #_Hmeta_pub & Hpub₂) & _ & HΦ)".
           injection Heq as <-.
           iDestruct (meta_agree with "Hmeta_pub _Hmeta_pub") as %<-. iClear "_Hmeta_pub".
-          iDestruct (inf_chaselev_pub_agree with "Hpub₁ Hpub₂") as %<-.
+          iDestruct (inf_chaselev_deque_pub_agree with "Hpub₁ Hpub₂") as %<-.
           (* do increment [front] *)
           wp_cmpxchg_suc.
           (* update front authority *)
-          iMod (inf_chaselev_front_auth_update (front2 + 1) with "Hfront_auth") as "Hfront_auth"; first lia.
+          iMod (inf_chaselev_deque_front_auth_update (front2 + 1) with "Hfront_auth") as "Hfront_auth"; first lia.
           (* emit front fragment at [front3 + 1] *)
           iClear "Hfront_frag".
-          iDestruct (inf_chaselev_front_frag_get with "Hfront_auth") as "#Hfront_frag".
+          iDestruct (inf_chaselev_deque_front_frag_get with "Hfront_auth") as "#Hfront_frag".
           (* update [pub] *)
-          iMod (inf_chaselev_pub_update [] with "Hpub₁ Hpub₂") as "(Hpub₁ & Hpub₂)".
+          iMod (inf_chaselev_deque_pub_update [] with "Hpub₁ Hpub₂") as "(Hpub₁ & Hpub₂)".
           (* end transaction *)
           iMod ("HΦ" with "[Hpub₂]") as "HΦ".
           { iRight. iExists [], v. iSplit; first done. repeat iExists _. naive_solver. }
@@ -1140,13 +1140,13 @@ Section inf_chaselev_GS.
           wp_bind (#l.(back) <- #(front2 + 1))%E.
           (* open invariant *)
           iInv "Hinv" as "(%front6 & %_back & %hist & %pub & %_priv & Hfront & Hback & >Hctl₁ & Hfront_auth & Harr_model & >%Hhist & Hhist_auth & Hpub₁ & Hstate)".
-          iDestruct (inf_chaselev_ctl_agree with "Hctl₁ Hctl₂") as %?. simplify- front6.
+          iDestruct (inf_chaselev_deque_ctl_agree with "Hctl₁ Hctl₂") as %?. simplify- front6.
           (* do increment [back] *)
           wp_store.
           (* update [back] in control tokens *)
-          iMod (inf_chaselev_ctl_update (front2 + 1) priv with "Hctl₁ Hctl₂") as "(Hctl₁ & Hctl₂)".
+          iMod (inf_chaselev_deque_ctl_update (front2 + 1) priv with "Hctl₁ Hctl₂") as "(Hctl₁ & Hctl₂)".
           (* from front fragment at [front2 + 1], we know [front2 + 1 ≤ front6] *)
-          iDestruct (inf_chaselev_front_valid with "Hfront_auth Hfront_frag") as %Hfront6.
+          iDestruct (inf_chaselev_deque_front_valid with "Hfront_auth Hfront_frag") as %Hfront6.
           (* hence, we are in state 2.2 *)
           iDestruct "Hstate" as "[%Hstate | (Hlock & [%Hstate | %Hstate])]"; [lia.. |].
           (* hence, [front6 = front2 + 1] *)
@@ -1168,7 +1168,7 @@ Section inf_chaselev_GS.
           wp_cmpxchg_fail; first naive_solver lia.
           (* emit front fragment at [front2 + 1] *)
           iClear "Hfront_frag".
-          iDestruct (inf_chaselev_front_frag_get with "Hfront_auth") as "#Hfront_frag".
+          iDestruct (inf_chaselev_deque_front_frag_get with "Hfront_auth") as "#Hfront_frag".
           (* close invariant *)
           iModIntro. iSplitL "Hfront Hback Hctl₁ Hfront_auth Harr_model Hhist_auth Hpub₁ Hlock".
           { iNext. iExists (front2 + 1), front2, hist, [], priv. iFrame. iSplit; first done.
@@ -1182,13 +1182,13 @@ Section inf_chaselev_GS.
           wp_bind (#l.(back) <- #(front2 + 1))%E.
           (* open invariant *)
           iInv "Hinv" as "(%front6 & %_back & %hist & %pub & %_priv & Hfront & Hback & >Hctl₁ & Hfront_auth & Harr_model & >%Hhist & Hhist_auth & Hpub₁ & Hstate)".
-          iDestruct (inf_chaselev_ctl_agree with "Hctl₁ Hctl₂") as %?. simplify- front6.
+          iDestruct (inf_chaselev_deque_ctl_agree with "Hctl₁ Hctl₂") as %?. simplify- front6.
           (* do increment [back] *)
           wp_store.
           (* update [back] in control tokens *)
-          iMod (inf_chaselev_ctl_update (front2 + 1) priv with "Hctl₁ Hctl₂") as "(Hctl₁ & Hctl₂)".
+          iMod (inf_chaselev_deque_ctl_update (front2 + 1) priv with "Hctl₁ Hctl₂") as "(Hctl₁ & Hctl₂)".
           (* from front fragment at [front 2 + 1], we know [front2 + 1 ≤ front6] *)
-          iDestruct (inf_chaselev_front_valid with "Hfront_auth Hfront_frag") as %Hfront6.
+          iDestruct (inf_chaselev_deque_front_valid with "Hfront_auth Hfront_frag") as %Hfront6.
           (* hence, we are in state 2.2 *)
           iDestruct "Hstate" as "[%Hstate | (Hlock & [%Hstate | %Hstate])]"; [lia.. |].
           (* hence, [front6 = front2 + 1] *)
@@ -1196,7 +1196,7 @@ Section inf_chaselev_GS.
           (* begin transaction *)
           iMod "HΦ" as "(%_pub & (%_l & %_γ_pub & %Heq & #_Hmeta_pub & Hpub₂) & _ & HΦ)". injection Heq as <-.
           iDestruct (meta_agree with "Hmeta_pub _Hmeta_pub") as %<-.
-          iDestruct (inf_chaselev_pub_agree with "Hpub₁ Hpub₂") as %<-.
+          iDestruct (inf_chaselev_deque_pub_agree with "Hpub₁ Hpub₂") as %<-.
           (* end transaction *)
           iMod ("HΦ" $! NONEV with "[Hpub₂]") as "HΦ".
           { iLeft. simplify. iSplit; first done. repeat iExists _. naive_solver. }
@@ -1215,7 +1215,7 @@ Section inf_chaselev_GS.
       + destruct Hstate as (Hstate & ->). assert (front3 = front2 + 1) as -> by lia.
         (* emit front fragment at [front2 + 1] *)
         iClear "Hfront_frag".
-        iDestruct (inf_chaselev_front_frag_get with "Hfront_auth") as "#Hfront_frag".
+        iDestruct (inf_chaselev_deque_front_frag_get with "Hfront_auth") as "#Hfront_frag".
         (* close invariant *)
         iModIntro. iSplitL "Hfront Hback Hctl₁ Hfront_auth Harr_model Hhist_auth Hpub₁ Hlock".
         { iNext. iExists (front2 + 1), front2, hist, [], priv. iFrame. iSplit; first done.
@@ -1234,13 +1234,13 @@ Section inf_chaselev_GS.
         wp_bind (#l.(back) <- #(front2 + 1)%nat)%E.
         (* open invariant *)
         iInv "Hinv" as "(%front4 & %_back & %hist & %pub & %_priv & Hfront & Hback & >Hctl₁ & Hfront_auth & Harr_model & >%Hhist & Hhist_auth & Hpub₁ & Hstate)".
-        iDestruct (inf_chaselev_ctl_agree with "Hctl₁ Hctl₂") as %?. simplify- front4.
+        iDestruct (inf_chaselev_deque_ctl_agree with "Hctl₁ Hctl₂") as %?. simplify- front4.
         (* do increment [back] *)
         wp_store.
         (* update [back] in control tokens *)
-        iMod (inf_chaselev_ctl_update (front2 + 1) priv with "Hctl₁ Hctl₂") as "(Hctl₁ & Hctl₂)".
+        iMod (inf_chaselev_deque_ctl_update (front2 + 1) priv with "Hctl₁ Hctl₂") as "(Hctl₁ & Hctl₂)".
         (* from front fragment at [front2 + 1], we know [front2 + 1 ≤ front4] *)
-        iDestruct (inf_chaselev_front_valid with "Hfront_auth Hfront_frag") as %Hfront4.
+        iDestruct (inf_chaselev_deque_front_valid with "Hfront_auth Hfront_frag") as %Hfront4.
         (* hence, we are in state 2.2 *)
         iDestruct "Hstate" as "[%Hstate | (Hlock & [%Hstate | %Hstate])]"; [lia.. |].
         (* hence, [front4 = front2 + 1] *)
@@ -1248,7 +1248,7 @@ Section inf_chaselev_GS.
         (* begin transaction *)
         iMod "HΦ" as "(%_pub & (%_l & %_γ_pub & %Heq & #_Hmeta_pub & Hpub₂) & _ & HΦ)". injection Heq as <-.
         iDestruct (meta_agree with "Hmeta_pub _Hmeta_pub") as %<-.
-        iDestruct (inf_chaselev_pub_agree with "Hpub₁ Hpub₂") as %<-.
+        iDestruct (inf_chaselev_deque_pub_agree with "Hpub₁ Hpub₂") as %<-.
         (* end transaction *)
         iMod ("HΦ" $! NONEV with "[Hpub₂]") as "HΦ".
         { iLeft. simplify. iSplit; first done. repeat iExists _. naive_solver. }
@@ -1280,13 +1280,13 @@ Section inf_chaselev_GS.
       }
       (* update [priv] in control tokens *)
       set (priv' := λ i, if decide (i = 0) then v else priv (i - 1)).
-      iMod (inf_chaselev_ctl_update (back - 1) priv' with "Hctl₁ Hctl₂") as "(Hctl₁ & Hctl₂)".
+      iMod (inf_chaselev_deque_ctl_update (back - 1) priv' with "Hctl₁ Hctl₂") as "(Hctl₁ & Hctl₂)".
       (* begin transaction *)
       iMod "HΦ" as "(%_pub & (%_l & %_γ_pub & %Heq & #_Hmeta_pub & Hpub₂) & (_ & HΦ))". injection Heq as <-.
       iDestruct (meta_agree with "Hmeta_pub _Hmeta_pub") as %<-. iClear "_Hmeta_pub".
-      iDestruct (inf_chaselev_pub_agree with "Hpub₁ Hpub₂") as %<-.
+      iDestruct (inf_chaselev_deque_pub_agree with "Hpub₁ Hpub₂") as %<-.
       (* update [pub] *)
-      iMod (inf_chaselev_pub_update pub' with "Hpub₁ Hpub₂") as "(Hpub₁ & Hpub₂)".
+      iMod (inf_chaselev_deque_pub_update pub' with "Hpub₁ Hpub₂") as "(Hpub₁ & Hpub₂)".
       (* end transaction *)
       iMod ("HΦ" with "[Hpub₂]") as "HΦ".
       { iRight. iExists pub', v. iSplit; first done. repeat iExists _. naive_solver. }
@@ -1326,13 +1326,13 @@ Section inf_chaselev_GS.
       wp_bind (!#l.(front))%E.
       (* open invariant *)
       iInv "Hinv" as "(%front3 & %_back & %hist & %pub & %_priv & Hfront & Hback & >Hctl₁ & Hfront_auth & Harr_model & >%Hhist & Hhist_auth & Hpub₁ & Hstate)".
-      iDestruct (inf_chaselev_ctl_agree with "Hctl₁ Hctl₂") as %?. simplify- front3.
+      iDestruct (inf_chaselev_deque_ctl_agree with "Hctl₁ Hctl₂") as %?. simplify- front3.
       (* do load [front] *)
       wp_load.
       (* we have lock, hence we are in state 1, hence [front3 ≤ back - 1] *)
-      iDestruct (inf_chaselev_lock_state with "Hlock Hstate") as %(Hfront3 & _).
+      iDestruct (inf_chaselev_deque_lock_state with "Hlock Hstate") as %(Hfront3 & _).
       (* emit front fragment at [front3] (to be used in branch 2.2) *)
-      iDestruct (inf_chaselev_front_frag_get with "Hfront_auth") as "#Hfront_frag".
+      iDestruct (inf_chaselev_deque_front_frag_get with "Hfront_auth") as "#Hfront_frag".
       (* close invariant *)
       iModIntro. iSplitL "Hfront Hback Hctl₁ Hfront_auth Harr_model Hhist_auth Hpub₁ Hstate".
       { repeat iExists _. iFrame. done. }
@@ -1349,11 +1349,11 @@ Section inf_chaselev_GS.
       awp_apply (inf_array_get_spec with "[//]") without "HΦ"; first lia.
       (* open invariant *)
       iInv "Hinv" as "(%front4 & %_back & %hist & %pub & %_priv & Hfront & Hback & >Hctl₁ & Hfront_auth & >Harr_model & >%Hhist & Hhist_auth & Hpub₁ & >Hstate)".
-      iDestruct (inf_chaselev_ctl_agree with "Hctl₁ Hctl₂") as %?. simplify- front4.
+      iDestruct (inf_chaselev_deque_ctl_agree with "Hctl₁ Hctl₂") as %?. simplify- front4.
       iAaccIntro with "Harr_model"; iIntros "Harr_model".
       { iModIntro. iFrame. iNext. repeat iExists _. iFrame. done. }
       (* we have lock, hence we are in state 1 *)
-      iDestruct (inf_chaselev_lock_state with "Hlock Hstate") as %Hstate.
+      iDestruct (inf_chaselev_deque_lock_state with "Hlock Hstate") as %Hstate.
       (* close invariant *)
       iModIntro. iSplitL "Hfront Hback Hctl₁ Hfront_auth Harr_model Hhist_auth Hpub₁ Hstate".
       { repeat iExists _. iFrame. done. }
@@ -1390,32 +1390,32 @@ Section inf_chaselev_GS.
         wp_bind (CmpXchg #l.(front) #front3 #(front3 + 1))%E.
         (* open invariant *)
         iInv "Hinv" as "(%front5 & %_back & %hist & %pub & %_priv & Hfront & Hback & >Hctl₁ & >Hfront_auth & Harr_model & >%Hhist & Hhist_auth & Hpub₁ & >Hstate)".
-        iDestruct (inf_chaselev_ctl_agree with "Hctl₁ Hctl₂") as %?. simplify- front5.
+        iDestruct (inf_chaselev_deque_ctl_agree with "Hctl₁ Hctl₂") as %?. simplify- front5.
         (* we have [front5 = front3] *)
         iAssert ⌜front5 = front3⌝%I as %->.
         { (* we have lock, hence we are in state 1 *)
-          iDestruct (inf_chaselev_lock_state with "Hlock Hstate") as %?.
+          iDestruct (inf_chaselev_deque_lock_state with "Hlock Hstate") as %?.
           (* from front fragment at [front3], we know [front3 ≤ front5] *)
-          iDestruct (inf_chaselev_front_valid with "Hfront_auth Hfront_frag") as %?.
+          iDestruct (inf_chaselev_deque_front_valid with "Hfront_auth Hfront_frag") as %?.
           iPureIntro. lia.
         }
         (* CAS must succeed *)
         wp_cmpxchg_suc.
         (* update front authority *)
-        iMod (inf_chaselev_front_auth_update (front3 + 1) with "Hfront_auth") as "Hfront_auth"; first lia.
+        iMod (inf_chaselev_deque_front_auth_update (front3 + 1) with "Hfront_auth") as "Hfront_auth"; first lia.
         (* emit front fragment at [front3 + 1] *)
         iClear "Hfront_frag".
-        iDestruct (inf_chaselev_front_frag_get with "Hfront_auth") as "#Hfront_frag".
+        iDestruct (inf_chaselev_deque_front_frag_get with "Hfront_auth") as "#Hfront_frag".
         (* we have lock, hence we are in state 1 *)
-        iDestruct (inf_chaselev_lock_state with "Hlock Hstate") as %(_ & Hpub).
+        iDestruct (inf_chaselev_deque_lock_state with "Hlock Hstate") as %(_ & Hpub).
         (* hence, [pub] is empty *)
         assert (length pub = 0) as ->%length_zero_iff_nil by lia. clear Hpub.
         (* update [hist] *)
         set (hist' := hist ++ [v]).
-        iAssert (inf_chaselev_hist_auth γ_hist hist' []) with "[> Hhist_auth]" as "Hhist_auth".
+        iAssert (inf_chaselev_deque_hist_auth γ_hist hist' []) with "[> Hhist_auth]" as "Hhist_auth".
         { iMod (mono_list_auth_own_update_app with "Hhist_auth") as "($ & _)". done. }
         (* update [priv] in control tokens *)
-        iMod (inf_chaselev_ctl_update front3 priv with "Hctl₁ Hctl₂") as "(Hctl₁ & Hctl₂)".
+        iMod (inf_chaselev_deque_ctl_update front3 priv with "Hctl₁ Hctl₂") as "(Hctl₁ & Hctl₂)".
         (* close invariant *)
         iModIntro. iSplitL "Hfront Hback Hctl₁ Hfront_auth Harr_model Hhist_auth Hpub₁ Hstate Hlock".
         { iNext. iExists (front3 + 1), front3, hist', [], priv. iFrame.
@@ -1447,13 +1447,13 @@ Section inf_chaselev_GS.
         wp_bind (#l.(back) <- #(front3 + 1))%E.
         (* open invariant *)
         iInv "Hinv" as "(%front6 & %_back & %hist & %pub & %_priv & Hfront & Hback & >Hctl₁ & Hfront_auth & Harr_model & >%Hhist & Hhist_auth & Hpub₁ & Hstate)".
-        iDestruct (inf_chaselev_ctl_agree with "Hctl₁ Hctl₂") as %?. simplify- front6.
+        iDestruct (inf_chaselev_deque_ctl_agree with "Hctl₁ Hctl₂") as %?. simplify- front6.
         (* do increment [back] *)
         wp_store.
         (* update [back] in control tokens *)
-        iMod (inf_chaselev_ctl_update (front3 + 1) priv with "Hctl₁ Hctl₂") as "(Hctl₁ & Hctl₂)".
+        iMod (inf_chaselev_deque_ctl_update (front3 + 1) priv with "Hctl₁ Hctl₂") as "(Hctl₁ & Hctl₂)".
         (* from front fragment at [front3 + 1], we know [front3 + 1 ≤ front6] *)
-        iDestruct (inf_chaselev_front_valid with "Hfront_auth Hfront_frag") as %Hfront6.
+        iDestruct (inf_chaselev_deque_front_valid with "Hfront_auth Hfront_frag") as %Hfront6.
         (* hence, we are in state 2.2 *)
         iDestruct "Hstate" as "[%Hstate | (Hlock & [%Hstate | %Hstate])]"; [lia.. |].
         (* hence, [front6 = front3 + 1] *)
@@ -1469,13 +1469,13 @@ Section inf_chaselev_GS.
 
         iApply "HΦ". repeat iExists _. iFrame "∗#". done.
   Qed.
-End inf_chaselev_GS.
+End inf_chaselev_deque_GS.
 
-#[global] Opaque inf_chaselev_make.
-#[global] Opaque inf_chaselev_push.
-#[global] Opaque inf_chaselev_steal.
-#[global] Opaque inf_chaselev_pop.
+#[global] Opaque inf_chaselev_deque_make.
+#[global] Opaque inf_chaselev_deque_push.
+#[global] Opaque inf_chaselev_deque_steal.
+#[global] Opaque inf_chaselev_deque_pop.
 
-#[global] Opaque inf_chaselev_inv.
-#[global] Opaque inf_chaselev_model.
-#[global] Opaque inf_chaselev_own.
+#[global] Opaque inf_chaselev_deque_inv.
+#[global] Opaque inf_chaselev_deque_model.
+#[global] Opaque inf_chaselev_deque_own.
